KitchenSink.v
@@ -18,6 +18,8 @@ Module KitchenSink(E : Embedding) (Lap: Laplace E) (LOGIC: APRHL E Lap).
       inc_cmd x ;;
       dec_cmd x.
 
+  Search welltyped.
+
   Goal forall ctx, VarMap.MapsTo x t_int ctx ->
                    VarMap.MapsTo y t_int ctx ->
                    welltyped ctx prog.
