Pattern.v
@@ -1,0 +1,210 @@
+Require Export Syntax.
+
+Definition uni_var := string.
+
+Inductive uni_res :=
+| uni_variable : var -> uni_res
+| uni_Z : Z -> uni_res
+| uni_positive : positive -> uni_res
+| uni_expr : expr -> uni_res
+| uni_base_instr : base_instr -> uni_res
+| uni_cmd : cmd -> uni_res.
+
+Lemma uni_res_eqdec : forall ur1 ur2 : uni_res,
+    {ur1 = ur2} + {ur1 <> ur2}.
+Proof.
+  destruct ur1.
+  - intros ur2; destruct ur2; prune_eqdec_cases.
+    destruct (var_eqdec v v0).
+    + subst; auto.
+    + right; intros contra; inversion contra; apply n; auto.
+  - intros ur2; destruct ur2; prune_eqdec_cases.
+    destruct (Z.eq_dec z z0).
+    + subst; auto.
+    + right; intros contra; inversion contra; apply n; auto.
+  - intros ur2; destruct ur2; prune_eqdec_cases.
+    destruct (Pos.eq_dec p p0).
+    + subst; auto.
+    + right; intros contra; inversion contra; apply n; auto.
+  - intros ur2; destruct ur2; prune_eqdec_cases.
+    destruct (expr_eqdec e e0).
+    + subst; auto.
+    + right; intros contra; inversion contra; apply n; auto.
+  - intros ur2; destruct ur2; prune_eqdec_cases.
+    destruct (base_instr_eqdec b b0).
+    + subst; auto.
+    + right; intros contra; inversion contra; apply n; auto.
+  - intros ur2; destruct ur2; prune_eqdec_cases.
+    destruct (cmd_eqdec c c0).
+    + subst; auto.
+    + right; intros contra; inversion contra; apply n; auto.
+Defined.
+
+Inductive atom_pat (T : Type) :=
+| apat_atom : T -> atom_pat T
+| apat_uni : uni_var -> atom_pat T.
+
+Definition var_pat := atom_pat var.
+Definition Z_pat := atom_pat Z.
+Definition positive_pat := atom_pat positive.
+
+Definition uni_env := VarMap.t uni_res.
+
+(* Produces either a list of disagreeing unification variables, or a union of
+   the two environments *)
+Definition uni_env_union' (e1 e2 : uni_env) : ((list uni_var) * uni_env) :=
+  VarMap.fold (fun uv ur acc =>
+                 match acc with
+                 | (bad_uvs, union) =>
+                   match VarMap.find uv union with
+                   | None => (bad_uvs, VarMap.add uv ur union)
+                   | Some ur2 => if uni_res_eqdec ur ur2
+                                then acc
+                                else (uv :: bad_uvs, union)
+                   end
+                 end)
+              e1
+              (@nil uni_var, e2).
+
+Definition M_uni := sum (list uni_var).
+Definition M_uni_return {T} (r : T) : M_uni T := inr r.
+Definition M_uni_bind {A B} (ma : M_uni A) (f : A -> M_uni B) : M_uni B :=
+  match ma with
+  | inl err => inl err
+  | inr a => f a
+  end.
+
+Notation "a '<-' ma ';;;' p" := (M_uni_bind ma (fun a => p))
+                                 (at level 75, right associativity) : M_uni_scope.
+Bind Scope M_uni_scope with M_uni.
+Delimit Scope M_uni_scope with M_uni.
+
+Definition uni_env_union (e1 e2 : uni_env) : M_uni uni_env :=
+  match uni_env_union' e1 e2 with
+  | (nil, union) => inr union
+  | (bad_uvs, _) => inl bad_uvs
+  end.
+
+Module TestUnion.
+  Definition build_uni_env_from_list (urs : list (uni_var * uni_res)) : uni_env :=
+    List.fold_right (fun uvur e =>
+                       VarMap.add (fst uvur) (snd uvur) e)
+                    (@VarMap.empty uni_res)
+                    urs.
+
+  Definition e1 := build_uni_env_from_list
+                     [("x"%string, uni_Z 1%Z);
+                        ("y"%string, uni_variable "k"%string)].
+
+  Definition e2 := build_uni_env_from_list
+                     [("x"%string, uni_Z 1%Z)].
+
+  Definition e3 := build_uni_env_from_list
+                     [("x"%string, uni_Z 2%Z);
+                        ("y"%string, uni_variable "k"%string)].
+
+  Eval compute in uni_env_union e1 e2.
+  Eval compute in uni_env_union e1 e3.
+
+  Definition test_val :=
+    (e1' <- M_uni_return e1 ;;;
+     e2' <- M_uni_return e2 ;;;
+     M_uni_return (e1', e2'))%M_uni.
+
+  Eval compute in test_val.
+
+End TestUnion.
+
+Inductive expr_pat :=
+| epat_wildcard : uni_var -> expr_pat
+| epat_var : var_pat -> expr_pat
+| epat_add : expr_pat -> expr_pat -> expr_pat
+| epat_minus : expr_pat -> expr_pat -> expr_pat
+| epat_mult : expr_pat -> expr_pat -> expr_pat
+| epat_div : expr_pat -> expr_pat -> expr_pat
+| epat_lt : expr_pat -> expr_pat -> expr_pat
+| epat_eq : expr_pat -> expr_pat -> expr_pat
+| epat_and : expr_pat -> expr_pat -> expr_pat
+| epat_or : expr_pat -> expr_pat -> expr_pat
+| epat_index : expr_pat -> expr_pat -> expr_pat
+| epat_length : expr_pat -> expr_pat.
+
+Definition match_var (vp : var_pat) (v : var) : uni_env -> M_uni uni_env :=
+  fun env =>
+  match vp with
+  | apat_atom _ v' => if var_eqdec v v'
+                   then M_uni_return env
+                   else inl []
+  | apat_uni _ uv => M_uni_return (VarMap.add uv (uni_variable v) env)
+  end.
+
+Fixpoint match_expr (ep : expr_pat) (e : expr) : uni_env -> M_uni uni_env :=
+  fun env =>
+    match ep, e with
+    | epat_wildcard x, _ => M_uni_return (VarMap.add x (uni_expr e) env)
+    | epat_var vp, e_var v => (
+        env' <- match_var vp v env ;;;
+        M_uni_return env'
+      )%M_uni
+    | epat_add ep1 ep2, e_add e1 e2 => (
+        env1 <- match_expr ep1 e1 env ;;;
+        env2 <- match_expr ep2 e2 env ;;;
+        uni_env_union env1 env2
+      )%M_uni
+    | epat_minus ep1 ep2, e_minus e1 e2 => (
+        env1 <- match_expr ep1 e1 env ;;;
+        env2 <- match_expr ep2 e2 env ;;;
+        uni_env_union env1 env2
+      )%M_uni
+    | epat_mult ep1 ep2, e_mult e1 e2 => (
+        env1 <- match_expr ep1 e1 env ;;;
+        env2 <- match_expr ep2 e2 env ;;;
+        uni_env_union env1 env2
+      )%M_uni
+    | epat_div ep1 ep2, e_div e1 e2 => (
+        env1 <- match_expr ep1 e1 env ;;;
+        env2 <- match_expr ep2 e2 env ;;;
+        uni_env_union env1 env2
+      )%M_uni
+    | epat_lt ep1 ep2, e_lt e1 e2 => (
+        env1 <- match_expr ep1 e1 env ;;;
+        env2 <- match_expr ep2 e2 env ;;;
+        uni_env_union env1 env2
+      )%M_uni
+    | epat_eq ep1 ep2, e_eq e1 e2 => (
+        env1 <- match_expr ep1 e1 env ;;;
+        env2 <- match_expr ep2 e2 env ;;;
+        uni_env_union env1 env2
+      )%M_uni
+    | epat_and ep1 ep2, e_and e1 e2 => (
+        env1 <- match_expr ep1 e1 env ;;;
+        env2 <- match_expr ep2 e2 env ;;;
+        uni_env_union env1 env2
+      )%M_uni
+    | epat_or ep1 ep2, e_or e1 e2 => (
+        env1 <- match_expr ep1 e1 env ;;;
+        env2 <- match_expr ep2 e2 env ;;;
+        uni_env_union env1 env2
+      )%M_uni
+    | epat_index ep1 ep2, e_index e1 e2 => (
+        env1 <- match_expr ep1 e1 env ;;;
+        env2 <- match_expr ep2 e2 env ;;;
+        uni_env_union env1 env2
+      )%M_uni
+    | epat_length ep1, e_length e1 =>
+        match_expr ep1 e1 env
+    | _, _ => inl []
+    end.
+
+Inductive bi_pat :=
+| bipat_wildcard : uni_var -> bi_pat
+| bipat_laplace : var_pat -> positive_pat -> expr_pat -> bi_pat
+| bipat_index_assign : var_pat -> expr_pat -> expr_pat -> bi_pat
+| bipat_length_assign : var_pat -> expr_pat -> bi_pat.
+
+Inductive cmd_pat :=
+| cpat_wildcard : uni_var -> cmd_pat
+| cpat_base_instr : bi_pat -> cmd_pat
+| cpat_cond : expr_pat -> cmd_pat -> cmd_pat -> cmd_pat
+| cpat_while : expr_pat -> cmd_pat -> cmd_pat
+| cpat_seq : cmd_pat -> cmd_pat -> cmd_pat.
